Structures/BlockMap.v
@@ -12,32 +12,33 @@ Require Import BlockChain FixedMap FixedList Parameters.
 Set Implicit Arguments.
 
 
-Definition blockmap_keytype := [eqType of Block].
-Definition blockmap_valuetype := [eqType of (bool * (ordinal N_rounds) )].
-Definition BlockMap := fixmap blockmap_keytype blockmap_valuetype  BlockHistory_size.
+Definition BlockMap_keytype := [eqType of Block].
+Definition BlockMap_valuetype := [eqType of (bool * (ordinal N_rounds) )].
+Definition BlockMap := fixmap BlockMap_keytype BlockMap_valuetype  BlockHistory_size.
 
-Definition blockmap_new : BlockMap := fixmap_empty blockmap_keytype blockmap_valuetype BlockHistory_size.
+Definition BlockMap_new : BlockMap := fixmap_empty BlockMap_keytype BlockMap_valuetype BlockHistory_size.
 
 
-Definition blockmap_find (bl : Block) (map : BlockMap) : option blockmap_valuetype := 
+Definition BlockMap_find (bl : Block) (map : BlockMap) : option BlockMap_valuetype := 
     fixmap_find bl map.
 
+Definition BlockMap_blocks (bmap : BlockMap) : seq (bool * nat) :=
+    map (fun pair => let: (b, or) := pair in (b, nat_of_ord or)) (fixlist_unwrap (fixmap_value bmap)).
 
-
-Definition blockmap_put_honest (bl : Block) (round: (ordinal N_rounds)) (map: BlockMap) :=
+Definition BlockMap_put_honest (bl : Block) (round: (ordinal N_rounds)) (map: BlockMap) :=
     fixmap_put (bl) (false, round) map.
         
-Definition blockmap_put_adversarial (bl : Block) (round : (ordinal N_rounds)) (map: BlockMap):=
+Definition BlockMap_put_adversarial (bl : Block) (round : (ordinal N_rounds)) (map: BlockMap):=
     fixmap_put (bl) (true, round) map.
 
 
-Definition blockmap_put_honest_on_success (o_bl : option Block) (round: (ordinal N_rounds)) (map: BlockMap) :=
+Definition BlockMap_put_honest_on_success (o_bl : option Block) (round: (ordinal N_rounds)) (map: BlockMap) :=
     match o_bl with
         | Some (bl) => fixmap_put (bl) (false, round) map
         | None => map
     end.        
 
-Definition blockmap_put_adversarial_on_success (o_bl : option Block) (round: (ordinal N_rounds)) (map: BlockMap) :=
+Definition BlockMap_put_adversarial_on_success (o_bl : option Block) (round: (ordinal N_rounds)) (map: BlockMap) :=
     match o_bl with
         | Some (bl) => fixmap_put (bl) (true, round) map
         | None => map
@@ -45,32 +46,32 @@ Definition blockmap_put_adversarial_on_success (o_bl : option Block) (round: (or
 
 
 
-  Definition blockmap_prod (m : BlockMap) := finmap_prod m.
-  Definition prod_blockmap pair : BlockMap := prod_finmap pair.
+  Definition BlockMap_prod (m : BlockMap) := finmap_prod m.
+  Definition prod_BlockMap pair : BlockMap := prod_finmap pair.
 
-  Lemma blockmap_cancel : cancel blockmap_prod prod_blockmap.
+  Lemma BlockMap_cancel : cancel BlockMap_prod prod_BlockMap.
   Proof.
     by case.
   Qed.
 
 
-  Definition blockmap_eqMixin  :=
-  CanEqMixin blockmap_cancel.
-  Canonical blockmap_eqType :=
-  Eval hnf in EqType BlockMap blockmap_eqMixin.
+  Definition BlockMap_eqMixin  :=
+  CanEqMixin BlockMap_cancel.
+  Canonical BlockMap_eqType :=
+  Eval hnf in EqType BlockMap BlockMap_eqMixin.
 
 
-  Definition blockmap_choiceMixin  :=
-  CanChoiceMixin blockmap_cancel.
-  Canonical blockmap_choiceType :=
-  Eval hnf in ChoiceType BlockMap blockmap_choiceMixin.
+  Definition BlockMap_choiceMixin  :=
+  CanChoiceMixin BlockMap_cancel.
+  Canonical BlockMap_choiceType :=
+  Eval hnf in ChoiceType BlockMap BlockMap_choiceMixin.
 
-  Definition blockmap_countMixin :=
-  CanCountMixin blockmap_cancel.
-  Canonical blockmap_countType :=
-  Eval hnf in CountType BlockMap blockmap_countMixin.
+  Definition BlockMap_countMixin :=
+  CanCountMixin BlockMap_cancel.
+  Canonical BlockMap_countType :=
+  Eval hnf in CountType BlockMap BlockMap_countMixin.
   
-  Definition blockmap_finMixin :=
-  CanFinMixin blockmap_cancel.
-  Canonical blockmap_finType :=
-  Eval hnf in FinType BlockMap blockmap_finMixin.
+  Definition BlockMap_finMixin :=
+  CanFinMixin BlockMap_cancel.
+  Canonical BlockMap_finType :=
+  Eval hnf in FinType BlockMap BlockMap_finMixin.
